pulse/lib/pulse/lib/Pulse.Lib.BigGhostReference.fsti
@@ -1,0 +1,92 @@
+(*
+   Copyright 2023 Microsoft Research
+
+   Licensed under the Apache License, Version 2.0 (the "License");
+   you may not use this file except in compliance with the License.
+   You may obtain a copy of the License at
+
+       http://www.apache.org/licenses/LICENSE-2.0
+
+   Unless required by applicable law or agreed to in writing, software
+   distributed under the License is distributed on an "AS IS" BASIS,
+   WITHOUT WARRANTIES OR CONDITIONS OF ANY KIND, either express or implied.
+   See the License for the specific language governing permissions and
+   limitations under the License.
+*)
+
+module Pulse.Lib.BigGhostReference
+open FStar.Tactics
+open Pulse.Lib.Core
+open PulseCore.FractionalPermission
+open FStar.Ghost
+
+[@@erasable]
+val ref ([@@@unused] a:Type u#2) : Type u#0
+      
+val gref_non_informative (a:Type u#2) : non_informative_witness (ref a)
+
+val pts_to (#a:Type)
+           (r:ref a)
+           (#[exact (`full_perm)] [@@@equate_by_smt] p:perm)
+           ([@@@equate_by_smt] n:a)
+: vprop
+
+val alloc (#a:Type) (x:a)
+  : stt_ghost (ref a) emp (fun r -> pts_to r x)
+  
+val read (#a:Type) (r:ref a) (#n:erased a) (#p:perm)
+  : stt_ghost (erased a)
+        (pts_to r #p n)
+        (fun x -> pts_to r #p n ** pure (n == x))
+
+val ( ! ) (#a:Type) (r:ref a) (#n:erased a) (#p:perm)
+  : stt_ghost (erased a)
+        (pts_to r #p n)
+        (fun x -> pts_to r #p n ** pure (n == x))
+
+
+val ( := ) (#a:Type) (r:ref a) (x:erased a) (#n:erased a)
+  : stt_ghost unit
+        (pts_to r n) 
+        (fun _ -> pts_to r x)
+
+let write = ( := )
+
+val free (#a:Type) (r:ref a) (#n:erased a)
+  : stt_ghost unit (pts_to r n) (fun _ -> emp)
+
+val share (#a:Type) (r:ref a) (#v:erased a) (#p:perm)
+  : stt_ghost unit
+      (pts_to r #p v)
+      (fun _ ->
+       pts_to r #(half_perm p) v **
+       pts_to r #(half_perm p) v)
+
+val gather (#a:Type) (r:ref a) (#x0 #x1:erased a) (#p0 #p1:perm)
+  : stt_ghost unit
+      (pts_to r #p0 x0 ** pts_to r #p1 x1)
+      (fun _ -> pts_to r #(sum_perm p0 p1) x0 ** pure (x0 == x1))
+
+(* Share/gather specialized to half permission *)
+val share2 (#a:Type) (r:ref a) (#v:erased a)
+  : stt_ghost unit
+      (pts_to r v)
+      (fun _ -> pts_to r #one_half v ** pts_to r #one_half v)
+
+val gather2 (#a:Type) (r:ref a) (#x0 #x1:erased a)
+  : stt_ghost unit
+      (pts_to r #one_half x0 ** pts_to r #one_half x1)
+      (fun _ -> pts_to r x0 ** pure (x0 == x1))
+
+val pts_to_injective_eq (#a:_)
+                        (#p #q:_)
+                        (#v0 #v1:a)
+                        (r:ref a)
+  : stt_ghost unit
+      (pts_to r #p v0 ** pts_to r #q v1)
+      (fun _ -> pts_to r #p v0 ** pts_to r #q v1 ** pure (v0 == v1))
+
+val pts_to_perm_bound (#a:_) (#p:_) (r:ref a) (#v:a)
+  : stt_ghost unit
+      (pts_to r #p v)
+      (fun _ -> pts_to r #p v ** pure (p `lesser_equal_perm` full_perm))
